fix STLC + sum + products

theories/logrel_heaplang_sessions/lty.v
@@ -39,20 +39,16 @@ End lty_ofe.
 
 Arguments ltyC : clear implicits.
 
-Section Classes.
-  Context {Σ : gFunctors}.
+(* Typing for operators *)
+Class LTyUnboxed `{Σ : gFunctors} (A : lty Σ) :=
+  lty_unboxed v : A v -∗ ⌜ val_is_unboxed v ⌝.
 
-  (* Typing for operators *)
-  Class LTyUnboxed (A : lty Σ) :=
-    lty_unboxed v : A v -∗ ⌜ val_is_unboxed v ⌝.
+Class LTyUnOp `{Σ : gFunctors} (op : un_op) (A B : lty Σ) :=
+  lty_un_op v : A v -∗ ∃ w, ⌜ un_op_eval op v = Some w ⌝ ∗ B w.
 
-  Class LTyUnOp (op : un_op) (A B : lty Σ) :=
-    lty_un_op v : A v -∗ ∃ w, ⌜ un_op_eval op v = Some w ⌝ ∗ B w.
+Class LTyBinOp `{Σ : gFunctors} (op : bin_op) (A1 A2 B : lty Σ) :=
+  lty_bin_op v1 v2 : A1 v1 -∗ A2 v2 -∗ ∃ w, ⌜ bin_op_eval op v1 v2 = Some w ⌝ ∗ B w.
 
-  Class LTyBinOp (op : bin_op) (A1 A2 B : lty Σ) :=
-    lty_bin_op v1 v2 : A1 v1 -∗ A2 v2 -∗ ∃ w, ⌜ bin_op_eval op v1 v2 = Some w ⌝ ∗ B w.
-
-  (* Copy types *)
-  Class LTyCopy (A : lty Σ) :=
-    lty_copy v :> Persistent (A v).
-End Classes.
+(* Copy types *)
+Class LTyCopy `{Σ : gFunctors} (A : lty Σ) :=
+  lty_copy v :> Persistent (A v).
