theories/logrel_heaplang_sessions/rules/basic.v
@@ -1,23 +1,28 @@
+From iris_examples.logrel_heaplang_sessions Require Export lty ltyping.
 From iris.heap_lang Require Export lifting metatheory.
 From iris.base_logic.lib Require Import invariants.
 From iris.heap_lang Require Import notation proofmode.
 
 Section types.
-  Context `{heapG Σ, lockG Σ, proto_chanG Σ}.
+  Context `{heapG Σ}.
 
   Definition lty_unit : lty Σ := Lty (λ w, ⌜ w = #() ⌝%I).
   Definition lty_bool : lty Σ := Lty (λ w, ∃ b : bool, ⌜ w = #b ⌝)%I.
   Definition lty_int : lty Σ := Lty (λ w, ∃ n : Z, ⌜ w = #n ⌝)%I.
+
 End types.
 
 Notation "()" := lty_unit : lty_scope.
 
-  (* Unboxed types *)
-  Global Instance lty_unit_unboxed : LTyUnboxed ().
+Section properties.
+  Context `{heapG Σ}.
+
+  (* TODO: Why doesn't Coq automatically infer the Σ from the context here? *)
+  Global Instance lty_unit_unboxed : @LTyUnboxed Σ ().
   Proof. by iIntros (v ->). Qed.
-  Global Instance lty_bool_unboxed : LTyUnboxed lty_bool.
+  Global Instance lty_bool_unboxed : @LTyUnboxed Σ lty_bool.
   Proof. iIntros (v). by iDestruct 1 as (b) "->". Qed.
-  Global Instance lty_int_unboxed : LTyUnboxed lty_int.
+  Global Instance lty_int_unboxed : @LTyUnboxed Σ lty_int.
   Proof. iIntros (v). by iDestruct 1 as (i) "->". Qed.
 
   Lemma ltyped_unit Γ : Γ ⊨ #() : ().
@@ -26,3 +31,4 @@ Notation "()" := lty_unit : lty_scope.
   Proof. iIntros (vs) "_ /=". iApply wp_value. rewrite /lty_car /=. eauto. Qed.
   Lemma ltyped_nat Γ (n : Z) : Γ ⊨ #n : lty_int.
   Proof. iIntros (vs) "_ /=". iApply wp_value. rewrite /lty_car /=. eauto. Qed.
+End properties.
