theories/logrel_heaplang_sessions/rules/prod.v
@@ -1,12 +1,24 @@
+From iris_examples.logrel_heaplang_sessions Require Export lty ltyping split arr.
+From iris.heap_lang Require Export lifting metatheory.
+From iris.base_logic.lib Require Import invariants.
+From iris.heap_lang Require Import notation proofmode.
+
+Section types.
+  Context `{heapG Σ}.
+
   Definition lty_prod (A1 A2 : lty Σ) : lty Σ := Lty (λ w,
     ∃ w1 w2, ⌜w = PairV w1 w2⌝ ∗ A1 w1 ∗ A2 w2)%I.
+End types.
 
 Infix "*" := lty_prod : lty_scope.
+
+Section properties.
+  Context `{heapG Σ}.
 
   Global Instance lty_prod_ne : NonExpansive2 (@lty_prod Σ).
   Proof. solve_proper. Qed.
 
-    Lemma ltyped_pair Γ Γ1 Γ2 e1 e2 A1 A2 :
+  Lemma ltyped_pair Γ Γ1 Γ2 e1 e2 A1 A2 :
     env_split Γ Γ1 Γ2 -∗ (Γ1 ⊨ e1 : A1) -∗ (Γ2 ⊨ e2 : A2) -∗ Γ ⊨ (e1,e2) : A1 * A2.
   Proof.
     iIntros "Hsplit H1 H2" (vs) "HΓ /=".
@@ -16,6 +28,7 @@ Infix "*" := lty_prod : lty_scope.
     wp_pures. iExists w1, w2. by iFrame.
   Qed.
 
+  (* TODO: use Any type to allow moving out one component of a pair *)
   Definition split : val := λ: "pair" "f", "f" (Fst "pair") (Snd "pair").
   Lemma ltyped_split Γ A1 A2 B:
     Γ ⊨ split : (A1 * A2 → (A1 → A2 → B) → B)%lty.
@@ -33,3 +46,5 @@ Infix "*" := lty_prod : lty_scope.
     iPoseProof ("Hg" with "Hw2") as "Hg".
     iFrame "Hg".
   Qed.
+
+End properties.
