theories/logrel_heaplang_sessions/rules/sum.v
@@ -1,7 +1,18 @@
+From iris_examples.logrel_heaplang_sessions Require Export lty.
+From iris.heap_lang Require Export lifting metatheory.
+From iris.base_logic.lib Require Import invariants.
+From iris.heap_lang Require Import notation proofmode.
+
+Section types.
+  Context `{heapG Σ}.
+
   Definition lty_sum (A1 A2 : lty Σ) : lty Σ := Lty (λ w,
     (∃ w1, ⌜w = InjLV w1⌝ ∗ A1 w1) ∨ (∃ w2, ⌜w = InjRV w2⌝ ∗ A2 w2))%I.
+End types.
 
 Infix "+" := lty_sum : lty_scope.
 
+Section properties.
   Global Instance lty_sum_ne : NonExpansive2 (@lty_sum Σ).
   Proof. solve_proper. Qed.
+End properties.
